\documentclass[12pt]{article}
\usepackage{latexsym}
\usepackage{amssymb,amsmath}
\usepackage[pdftex]{graphicx}
\usepackage{listings}
\usepackage{xcolor}
\lstset{language=R,basicstyle=\scriptsize\ttfamily,commentstyle=\ttfamily\color{gray},frame=single,breaklines=true,keepspaces = true,keywordstyle=\color{red},xleftmargin=-10mm}


\topmargin = 0.1in \textwidth=5.7in \textheight=8.6in

\oddsidemargin = 0.2in \evensidemargin = 0.2in


\begin{document}


\begin{center}
Proof 9-2 \\
Larson Hogstrom - Math E156 - 2014
\end{center}



Poisson distribution as the limit of a binomial distribution

\paragraph*{}

Random variable $X_n$ has a binomial distribution with parameters $n$ and $p$, expectation $\lambda = np$. So $p = \lambda / n.$

Its mass function is $$P(X_n = x) = \binom{n}{x}p^x(1-p)^{n-x}=  \frac{n!}{x!(n-x)!} \frac{\lambda^x}{n^x} (1-\frac{\lambda}{n})^{n-x}.$$

Take the limit as $n \rightarrow \infty$ to get the mass function for a Poisson random variable $X$:
$$P(X = x) = e^{-\lambda}\frac{\lambda^x}{x!}.$$

Solution:


$$ \lim_{n\to\infty} \frac{n!}{x!(n-x)!} \frac{\lambda^x}{n^x} (1-\frac{\lambda}{n})^{n-x}$$
$$ \lim_{n\to\infty} \frac{n(n-1)(n-2)..(n-x+1)!}{x!} \frac{\lambda^x}{n^x} (1-\frac{\lambda}{n})^{n-x}$$



\begin{itemize}
\item $ n(n-1)(n-2)...(n-x + 1) =  n^x + 0(n^{x-1}) $
\item $ \lim_{n\to\infty} \frac{n(n-1)(n-2)...(n-x + 1)}{n^x x!} = \frac{1}{x!} $
\\ \\
Now
$$ \lim_{n\to\infty} \frac{\lambda^x}{x!} (1-\frac{\lambda}{n})^{n}(1-\frac{\lambda}{n})^{-x}$$

\item $ \lim_{n\to\infty} (1 - \frac{\lambda}{n})^n = e^{-\lambda}$
\item $ \lim_{n\to\infty} (1 - \frac{\lambda}{n})^{-x} = 1$
\end{itemize}
$$ \lim_{n\to\infty} \frac{\lambda^x}{x!} e^{-\lambda} = Pois(\lambda) $$ 

\paragraph*{}
$ source: http://en.wikipedia.org/wiki/Poisson_limit_theorem $
\end{document}
