\documentclass[12pt]{article}
\usepackage{latexsym}
\usepackage{amssymb,amsmath}
\usepackage[pdftex]{graphicx}
\usepackage{listings}
\usepackage{xcolor}
\lstset{language=R,basicstyle=\scriptsize\ttfamily,commentstyle=\ttfamily\color{gray},frame=single,breaklines=true,keepspaces = true,keywordstyle=\color{red},xleftmargin=-10mm}


\topmargin = 0.1in \textwidth=5.7in \textheight=8.6in

\oddsidemargin = 0.2in \evensidemargin = 0.2in


\begin{document}


\begin{center}
Proof 4-3 \\
Larson Hogstrom - Math E156 - 2014
\end{center}





Prove that the Poisson distribution with parameter $\lambda$ has mean and variance both equal to $\lambda$. 
Solution:

$$ E[X] = \sum_{x=0}^{\infty}  x \frac{e^{-\lambda}\lambda^x}{x!} $$
$$ E[X] = \sum_{x=1}^{\infty}  x \frac{e^{-\lambda}\lambda^x}{x!} $$
$$ E[X] = \sum_{x=1}^{\infty}  \frac{e^{-\lambda}\lambda^x}{(x-1)!} $$
$$ E[X] = \sum_{x=1}^{\infty}  \frac{e^{-\lambda}\lambda\lambda^{x-1}}{(x-1)!} $$
$$ E[X] = e^{-\lambda}\lambda \sum_{x=1}^{\infty}  \frac{\lambda^{x-1}}{(x-1)!} $$
let k = x-1
$$ E[X] = e^{-\lambda}\lambda \sum_{k=1}^{\infty}  \frac{\lambda^k}{k!} $$
$$ E[X] = e^{-\lambda}\lambda e^\lambda = \lambda$$
* Taylor Series expansion of exponential function

\pagebreak

\paragraph*{}
Prove that if $X_1$ and $X_2$ are independent Poisson random variables with parameters $\lambda_1$ and $\lambda_2$ respectively, then $X_1 + X_2$ is Poisson with parameter $\lambda_1 + \lambda_2$.


$$ P(X_1 + X_2 = m) = \sum_{j=0}^m P(X_1 = j)P(X_2 = m-j) $$
$$ = \sum_{j=0}^m e^{-\lambda_1}\frac{\lambda_1^j}{j!}  e^{-\lambda_2}  \frac{\lambda_2^{m-j}}{(m-j)!} $$
$$ = \sum_{j=0}^m  e^{-(\lambda_1 + \lambda_2)} \frac{\lambda_1^j}{j!}    \frac{\lambda_2^{m-j}}{(m-j)!} $$
$$ = \frac{e^{-(\lambda_1 + \lambda_2)}}{m!} \sum_{j=0}^m  \frac{m!}{j!(m-j)!} \lambda_1^j \lambda_2^{m-j}$$ 
*Binomial to obtain $( \lambda_1 + \lambda_2 )^m $
$$ = \frac{e^{-(\lambda_1 + \lambda_2)}}{m!} ( \lambda_1 + \lambda_2 )^m $$




\end{document}
